\begin{definition}
    The \textbf{Fourier series} of a function $f$ is given by 
    \begin{equation*}
        Sf(x) = \frac{a_0}{2} + \sum_{k=1}^\infty a_k \cos(kx) + b_k \sin(kx),
    \end{equation*}
    where the \textbf{Fourier coefficients} $a_k$ and $b_k$ are 
    given by 
    \begin{equation*}
        a_k = \frac{1}{\pi} \int_{-\pi}^\pi f(x) \cos(kx)dx, \quad
        b_k = \frac{1}{\pi} \int_{-\pi}^\pi f(x) \sin(kx)dx.
    \end{equation*}
    Or, alternatively, 
    \begin{equation*}
        Sf(x) = \sum_{k=-\infty}^\infty c_k e^{ikx},
    \end{equation*}
    where the \textbf{Fourier coefficients} $c_k$ are given by
    \begin{equation*}
        c_k = \frac{1}{2\pi} \int_{-\pi}^\pi f(x) e^{-ikx}dx.
    \end{equation*}
\end{definition}

\begin{definition}
    The \textbf{Truncated Fourier series} of a function $f$ is denoted by 
    \begin{equation*}
        S_N f(x) = \frac{a_0}{2} + \sum_{k=1}^N a_k \cos(kx) + b_k \sin(kx) = \sum_{k=-N}^N c_k e^{ikx}.
    \end{equation*}
\end{definition}

\begin{proposition}
    Let $a_k$ and $b_k$ be the Fourier coefficients of a function $f$. Then 
    \begin{thmenum}
        \item If $f\in\L^1$, $\abs{a_k}, \abs{b_k}\leq C\norm{f}_1$ for some constant $C>0$.
        \item If $f\in\L^\infty$, $\abs{a_k}, \abs{b_k}\leq C\norm{f}_\infty$ for some constant $C>0$.
    \end{thmenum}
\end{proposition}
\begin{proof}
    To see (a), compute that
    \begin{equation*}
        \abs{a_k} \leq \frac{1}{\pi}\int_{-\pi}^\pi \abs{f(x)}\abs{\cos(kx)}dx \leq \frac{1}{\pi}\int_{-\pi}^\pi \abs{f(x)}dx = C\norm{f}_1
    \end{equation*}
    and similarly for $b_k$. 
    For (b), 
    \begin{equation*}
        \abs{a_k} \leq \frac{1}{\pi}\int_{-\pi}^\pi \abs{f(x)}\abs{\cos(kx)}dx \leq \frac{1}{\pi}\int_{-\pi}^\pi \norm{f}_\infty dx = 2\norm{f}_\infty = C\norm{f}_\infty.
    \end{equation*}
    The proof for $b_k$ is analogous.
\end{proof}

\begin{lemma}[Riemann-Lebesgue \rom{1}]
    Let $f\in \L^1[a,b]$. Then 
    \begin{equation*}
        \lim_{n\to\infty} \int_a^b f(x)e^{-inx}dx = 0.
    \end{equation*}
\end{lemma}
\begin{proof}
    Let $\epsilon > 0$. Since $f\in\L^1[a,b]$, there is a step function 
    $g$ such that $\norm{f-g}_1 < \epsilon$. For any interval $E$, 
    \begin{equation*}
        \abs{\int_a^b \chi_E(x)e^{-inx}dx} \leq \abs{\int_E \cos(nx)dx} + \abs{\int_E \sin(nx)dx} 
        \leq \frac{2\pi}{n} \to 0
    \end{equation*}
    as $n\to\infty$. A step function is a linear combination of characteristic 
    functions of intervals, and thus $\abs{\int_a^b g(x)e^{-inx}dx} \to 0$ as $n\to\infty$.
    Therefore, 
    \begin{equation*}
        \begin{split}
            \abs{\int_a^b f(x)e^{-inx}dx} &\leq \abs{\int_a^b (f(x)-g(x))e^{-inx}dx} + \abs{\int_a^b g(x)e^{-inx}dx} \\
            &\leq \norm{f-g}_1 + \abs{\int_a^b g(x)e^{-inx}dx} \to 0
        \end{split}
    \end{equation*}
    as $n\to\infty$.
\end{proof}

\begin{definition}
    The space of piecewise continuous functions on $[a,b]$ is denoted by $PC[a,b]$. 
    The symbol $PC^n[a,b]$ denotes the space of functions having continuous derivatives up to order $n-1$, 
    with the $n$-th derivative being piecewise continuous.
\end{definition}

\begin{proposition}
    Let $f\in PC^1[-\pi,\pi]$ and 
    \begin{equation*}
        f(x) = \frac{a_0}{2} + \sum_{k=1}^\infty a_k \cos(kx) + b_k \sin(kx).
    \end{equation*}
    Then 
    \begin{equation*}
        f'(x) = \sum_{k=1}^\infty -ka_k \sin(kx) + kb_k \cos(kx).
    \end{equation*}
\end{proposition}
\begin{proof}
    Differentiation term by term gives the desired result.
\end{proof}
\begin{remark}
    If $f\in PC^n[-\pi,\pi]$, then
    \begin{equation*}
        \abs{a_k}, \abs{b_k} \leq \frac{\norm{f}_{PC^n}}{k^n},
    \end{equation*}
    where $\norm{f}_{PC^n} = \sum_{j=0}^n \norm{f^{(j)}}_\infty$.
\end{remark}

\begin{definition}
    Let $f$ be a function on $\R$. The \textbf{right-limit} and 
    the \textbf{left-limit} of $f$ at $x$ are defined by
    \begin{equation*}
        f(x^+) = \lim_{h\to 0^+} f(x+h), \quad f(x^-) = \lim_{h\to 0^+} f(x-h).
    \end{equation*}
\end{definition}

\begin{definition}
    A \textbf{kernel} is a function $k:X\times X\to\R$ such that 
    \begin{thmenum}
        \item $k(x,y) = k(y,x)$ for all $x,y\in X$,
        \item For finitely many points $x_1,\ldots,x_n\in X$ and scalars $a_1,\ldots,a_n\in\R$, 
        \begin{equation*}
            \sum_{i=1}^n \sum_{j=1}^n a_ia_jk(x_i,x_j) \geq 0.
        \end{equation*}
    \end{thmenum}
\end{definition}

\begin{definition}
    The \textbf{Dirichlet kernel} is defined by
    \begin{equation*}
        D_N(x) = \frac{1}{2\pi}\sum_{k=-N}^N e^{ikx}.
    \end{equation*}
\end{definition}
\begin{remark}
    The Dirichlet kernel can be simplified to 
    \begin{equation*}
        D_N(x) = \frac{\sin\pth{(N+1/2)x}}{2\pi\sin(x/2)}.
    \end{equation*}
    To see this, note that 
    \begin{equation*}
        2\pi D_N(x)(e^{ix}-1) = e^{i(N+1)x} - e^{-iNx} 
        = \frac{e^{i(N+1/2)x} - e^{-i(N+1/2)x}}{e^{ix/2} - e^{-ix/2}}.
    \end{equation*}
    And thus,
    \begin{equation*}
        D_N(x) = \frac{\sin\pth{(N+1/2)x}}{2\pi\sin(x/2)}.
    \end{equation*}
    Some other properties of the Dirichlet kernel include $D_N(-x) = D_N(x)$ 
    and $\int_{-\pi}^\pi D_N(x)dx = 1$.
\end{remark}

\begin{definition}
    Let $f,g:X\to\R$. The \textbf{convolution} of $f$ and $g$ is defined by
    \begin{equation*}
        (f*g)(x) = \int_X f(x-y)g(y)dy.
    \end{equation*}
\end{definition}

\begin{proposition}
    For any $2\pi$-periodic function $f\in PC$,
    \begin{equation*}
        S_Nf = D_N*f.
    \end{equation*}
\end{proposition}
\begin{proof}
    Compute that 
    \begin{equation*}
        \begin{split}
            S_Nf(x) &= \sum_{k=-N}^N c_k e^{ikx} = \sum_{k=-N}^N \frac{1}{2\pi} \int_{-\pi}^\pi f(y)e^{-iky}dy e^{ikx} \\
            &= \int_{-\pi}^\pi f(y) \frac{1}{2\pi}\sum_{k=-N}^N e^{ik(x-y)}dy = \int_{-\pi}^\pi f(y)D_N(x-y)dy = (D_N*f)(x).
        \end{split}
    \end{equation*}
\end{proof}

\begin{theorem}[Dirichlet-Jordan]
    Let $f$ be a $2\pi$-periodic function and piecewise Lipschitz. Then 
    \begin{equation*}
        \lim_{N\to\infty} S_Nf(x) = \frac{f(x^+)+f(x^-)}{2}.
    \end{equation*}
    In particular, if $f$ is continuous at $x$, then 
    \begin{equation*}
        \lim_{N\to\infty} S_Nf(x) = f(x).
    \end{equation*}
\end{theorem}
\begin{proof}
    Since $f$ is $2\pi$-periodic,
    \begin{equation*}
        \begin{split}
            S_Nf(x) &= \int_{-\pi}^\pi D_N(x-y)f(y)dy = \int_{-\pi}^\pi D_N(y)f(x-y)dy \\
            &= \int_0^\pi D_N(y)f(x-y)dy + \int_{-\pi}^0 D_N(y)f(x-y)dy \\
            &= \int_0^\pi D_N(y)f(x-y)dy + \int_0^\pi D_N(-y)f(x+y)dy \\
            &= \int_0^\pi D_N(y)\pth{f(x-y)+f(x+y)}dy.
        \end{split}
    \end{equation*}
    Notice that 
    \begin{equation*}
        \frac{1}{2}\pth{f(x^+)+f(x^-)} = \int_0^\pi D_N(y)\pth{f(x^+)+f(x^-)}dy.
    \end{equation*}
    Thus for given $x$, we have 
    \begin{equation*}
        \begin{split}
            \abs{S_Nf(x) - \frac{f(x^+)+f(x^-)}{2}} &\leq \abs{\int_0^\pi D_N(y)\pth{f(x+y)-f(x^+)}dy} \\
            &\quad + \abs{\int_0^\pi D_N(y)\pth{f(x-y)-f(x^-)}dy}.
        \end{split}
    \end{equation*}
    We claim that 
    \begin{equation*}
        \int_0^\pi D_N(y)\abs{f(x+y)-f(x^+)}dy \to 0
    \end{equation*}
    as $N\to\infty$ and the other integral is similar. There is a $\delta>0$ such that 
    $f$ is continuous on $[x,x+\delta]$. Thus $f$ is uniformly continuous on 
    $[x,x+\delta]$, and $\abs{f(x+y)-f(x^+)} < Cy$ for some constant $C>0$ and 
    $y\in[0,\delta]$. Then 
    \begin{equation*}
        \int_0^\delta \abs{D_N(y)}\abs{f(x+y)-f(x^+)}dy \leq C\int_0^\delta y\abs{D_N(y)}dy
        \leq C\int_0^\delta dy = C\delta, 
    \end{equation*}
    because $\abs{D_N(t)}\leq 1/\abs{t}$. On the other hand, 
    \begin{equation*}
        \begin{split}
            \int_\delta^\pi \abs{D_N(y)}\abs{f(x+y)-f(x^+)}dy 
            &\leq \frac{1}{2\pi}\int_\delta^\pi \frac{\sin((N+1/2)y)}{\sin(y/2)}\abs{f(x+y)-f(x^+)}dy \\
            &\leq \frac{1}{2\pi\sin(\delta/2)}\int_\delta^\pi \sin((N+1/2)y)g(y)dy \to 0,
        \end{split}
    \end{equation*}
    as $N\to\infty$ by the Riemann-Lebesgue lemma, where $g(y) = \abs{f(x+y)-f(x^+)}$ 
    is a continuous function on $[\delta,\pi]$. Hence we have
    \begin{equation*}
        \abs{\int_0^\pi D_N(y)\pth{f(x+y)-f(x^+)}dy} \to 0 \quad \text{as } N\to\infty.
    \end{equation*}
    We now see that 
    \begin{equation*}
        \abs{S_Nf(x) - \frac{f(x^+)+f(x^-)}{2}} \to 0 \quad \text{as } N\to\infty.
    \end{equation*}
    The pointwise convergence is achieved whenever $f$ is continuous since 
    $f(x^+)=f(x^-)=f(x)$.
\end{proof}

\begin{definition}
    The series $\sigma_Nf$ is defined by 
    \begin{equation*}
        \sigma_Nf(x) = \frac{1}{N+1}\sum_{n=0}^{N} S_nf(x).
    \end{equation*}
\end{definition}
\begin{remark}
    The series $\sigma_Nf$ is the Cesaro's mean of the Fourier series of $f$.
\end{remark}

\begin{definition}
    The \textbf{Fejer kernel} is defined by 
    \begin{equation*}
        F_N(x) = \frac{1}{N+1}\sum_{k=0}^N D_k(x).
    \end{equation*}
\end{definition}
\begin{remark}
    The Fejer kernel can be simplified to 
    \begin{equation*}
        F_N(x) = \frac{\sin^2\pth{\frac{N+1}{2}x}}{2\pi(N+1)\sin^2(x/2)}.
    \end{equation*}
    To see this, note that 
    \begin{equation*}
        \begin{split}
            F_N(t) &= \frac{1}{N+1}\sum_{k=0}^{N} D_k(t) 
            = \frac{1}{2\pi(N+1)}\sum_{k=0}^{N} \frac{\sin((k+1/2)t)}{\sin(t/2)} \\
            &= \frac{1}{2\pi(N+1)\sin^2(t/2)}\sum_{k=0}^{N} \sin((k+1/2)t)\sin(t/2) \\
            &= \frac{1}{2\pi(N+1)\sin^2(t/2)}\sum_{k=0}^{N} \cos(kt) - \cos((k+1)t) \\ 
            &= \frac{1}{4\pi(N+1)\sin^2(t/2)}\pth{1 - \cos((N+1)t)}
            = \frac{\sin^2\pth{\frac{N+1}{2}t}}{2\pi(N+1)\sin^2(t/2)}.
        \end{split}
    \end{equation*}
    Some other properties of the Fejer kernel include that if $f = 1$, then 
    \begin{equation*}
        \sigma_Nf = \int_{-\pi}^{\pi} F_N(x)dx = 1,
    \end{equation*}
    and that $F_N(-x) = F_N(x), F_N \geq 0$. Also, 
    \begin{equation*}
        \sigma_Nf(x) = \frac{1}{N+1}\sum_{k=0}^{N} \int_{-\pi}^\pi D_k(x-y)f(y)dy
        = \int_{-\pi}^\pi \pth{\frac{1}{N+1}\sum_{k=0}^{N}D_k(x-y)}f(y)dy
        = F_N*f(x).
    \end{equation*}
\end{remark}

\begin{definition}
    $C_{2\pi}$ denote the space of $2\pi$-periodic continuous functions. 
    $C^k_{2\pi}$ denotes the space of $2\pi$-periodic functions having continuous 
    derivatives up to order $k$.
\end{definition}

\begin{theorem}[Fejer]
    Let $f\in C_{2\pi}$. Then $\sigma_Nf \to f$ uniformly.
\end{theorem}
\begin{proof}
    Let $\epsilon>0$. There is a $\delta>0$ such that $\abs{f(x)-f(y)}<\epsilon$ 
    whenever $\abs{x-y}<\delta$. Observe that if $\abs{t}\geq\delta$, then 
    \begin{equation*}
        F_N(t) \leq \frac{1}{2\pi(N+1)\sin^2(\delta/2)} \to 0
    \end{equation*}
    as $N\to\infty$. Hence 
    \begin{equation*}
        \begin{split}
            \abs{\sigma_Nf(x) - f(x)} &= \abs{\int_{-\pi}^\pi F_N(x-y)f(y)dy - f(x)}  
            \leq \int_{-\pi}^\pi F_N(x-y)\abs{f(y)-f(x)}dy \\
            &\leq \int_{\abs{x-y}\leq \delta} F_N(x-y)\abs{f(y)-f(x)}dy + \int_{\delta\leq\abs{x-y}\leq\pi} F_N(x-y)\abs{f(y)-f(x)}dy \\
            &\leq \epsilon\int_{-\pi}^\pi F_N(x-y)dy + 2\norm{f}_\infty\int_{\delta\leq\abs{x-y}\leq\pi} F_N(x-y)dy \\
            &= \epsilon + 2\norm{f}_\infty\frac{\pi-\delta}{2\pi(N+1)\sin^2(\delta/2)} \to 0
        \end{split}
    \end{equation*}
    as $N\to\infty$.
\end{proof}

\begin{definition}
    The \textbf{trigonometric polynomial} of degree $N$ is a function of the form 
    \begin{equation*}
        TP_N(x) = \sum_{k=0}^N a_k\cos(kx) + b_k\sin(kx). 
    \end{equation*}
    The \textbf{trigonometric polynomial space} is denoted by $TP = \cup_N TP_N$.
\end{definition}

\begin{theorem}
    Under $\L^2[-\pi,\pi]$, $PC_{2\pi}\subset\overline{TP}$.
\end{theorem}
\begin{proof}
    Since continuous functions are dense in $PC_{2\pi}$, it suffices to show 
    that continuous functions can be approximated by trigonometric polynomials.
    Let $f\in C_{2\pi}$. By the Fejer theorem, $\sigma_Nf \to f$ uniformly.
    Since $\sigma_Nf$ is a trigonometric polynomial, $f$ can be approximated
    by trigonometric polynomials. 
\end{proof}

\begin{definition}
    The \textbf{best approximation error} of a function $f$ by a trigonometric 
    polynomial is defined by $\tilde{E}_N(f) = \inf_{p\in TP_N}\norm{p-f}_\infty$. 
\end{definition}

\begin{theorem}\label{thm:fourier_series_approx_loss}
    For $f\in C_{2\pi}$, 
    \begin{equation*}
        \norm{S_Nf - f}_\infty \leq C(1+\log N)\tilde{E}_N(f)
    \end{equation*}
    for some constant $C>0$.
\end{theorem}
\begin{proof}
    Recall that $S_Nf = D_N*f$. Then
    \begin{equation*}
        \abs{S_Nf(x)} = \abs{\int_{-\pi}^\pi D_N(x-y)f(y)dy} \leq \int_{-\pi}^\pi \abs{D_N(x-y)}\abs{f(y)}dy
        \leq \norm{f}_\infty\int_{-\pi}^\pi \abs{D_N(t)}dt.
    \end{equation*}
    Observe that 
    \begin{equation*}
        \abs{D_N(t)} = \frac{1}{2\pi}\abs{\frac{\sin\pth{(N+1/2)t}}{\sin(t/2)}} \leq \min\set{\frac{2N+1}{2\pi}, \frac{1}{2\abs{t}}}.
    \end{equation*}
    Thus 
    \begin{equation*}
        \begin{split}
            \int_{-\pi}^{\pi} \abs{D_N(t)}dt &\leq \int_{\abs{t}\leq \pi/(2N+1)} \frac{2N+1}{2\pi}dt + \int_{\pi/(2N+1)\leq\abs{t}\leq\pi} \frac{1}{2\abs{t}}dt \\
            &\leq \frac{2N+1}{2\pi}\frac{2\pi}{2N+1} + 2\cdot\frac{1}{2}\log(2N+1) \leq C(1 + \log N)
        \end{split}
    \end{equation*}
    for some constant $C>0$. Now let $q^*$ be the best approximation to $f$ in $TP_N$. 
    Notice that $S_Nq^* = q^*$ and $S_N$ is a linear operator. Then 
    \begin{equation*}
        \norm{S_Nf - q^*}_\infty = \norm{S_Nf - S_Nq^*}_\infty 
        \leq \norm{S_N}\norm{f-q^*}_\infty \leq C(1+\log N)\tilde{E}_N(f)
    \end{equation*}
    as desired.
\end{proof}

\begin{theorem}
    If $f\in C_{2\pi}$ is $L$-Lipschitz, then
    \begin{thmenum}
        \item $\norm{\sigma_Nf - f}_\infty \leq C_1\frac{1+\log N}{N}L$
        \item $\norm{S_Nf - f}_\infty \leq C_2\frac{(1+\log N)^2}{N}L$
    \end{thmenum}
    for some constant $C_1,C_2>0$.
\end{theorem}
\begin{proof}
    For (a) we have 
    \begin{equation*}
        \sigma_Nf(x) = (F_N*f)(x) = \int_{-\pi}^\pi F_N(x-y)f(y)dy.
    \end{equation*}
    And thus
    \begin{equation*}
        \begin{split}
            \abs{\sigma_Nf(x) - f(x)} &\leq \int_{-\pi}^\pi F_N(x-y)\abs{f(y)-f(x)}dy \\
            &= \int_{-\pi}^\pi F_N(u)\abs{f(x-u)-f(x)}du \leq L\int_{-\pi}^\pi F_N(u)\abs{u}du.
        \end{split}
    \end{equation*}
    Observe that 
    \begin{equation*}
        \abs{F_N(u)} = \frac{1}{2\pi(N+1)}\abs{\frac{\sin^2\pth{\frac{N+1}{2}u}}{\sin^2(u/2)}} 
        \leq \min\set{\frac{N+1}{2\pi}, \frac{\pi}{2(N+1)\abs{u}^2}}.
    \end{equation*}
    Then 
    \begin{equation*}
        \begin{split}
            L\int_{-\pi}^\pi F_N(u)\abs{u}du &\leq L\int_{\abs{u}\leq \pi/(N+1)} \frac{N+1}{2\pi}\abs{u}du + L\int_{\pi/(N+1)\leq\abs{u}\leq\pi} \frac{\pi}{2(N+1)\abs{u}^2}\abs{u}du \\
            &\leq L\int_{\abs{u}\leq \pi/(N+1)} \frac{N+1}{2\pi}\frac{\pi}{N+1}du + \frac{L\pi}{2(N+1)}\cdot 2\log(N+1) \\
            &= \frac{L\pi}{N+1} + L\pi\frac{\log(N+1)}{N+1} \leq C_1\frac{1+\log N}{N}L
        \end{split}
    \end{equation*}
    for some constant $C_1>0$. 
    
    For (b), from \cref{thm:fourier_series_approx_loss} we have
    \begin{equation*}
        \norm{S_Nf - f}_\infty \leq C(1+\log N)\tilde{E}_N(f) 
        \leq C(1+\log N)\norm{\sigma_Nf - f}_\infty \leq C_2\frac{(1+\log N)^2}{N}L
    \end{equation*}
    for some constant $C_2>0$.
\end{proof}
