\begin{definition}
    Let $\set{M_n}\subset B(X,Y)$ be a sequence of bounded linear operators. $M_n$ 
    \textbf{converges strongly} if for any $x\in X$, $\norm{M_nx - y}_Y\to 0$ for some $y\in Y$.
\end{definition}

\begin{proposition}
    If $\set{M_n}\subset B(X,Y)$ converges strongly, then there is an $M\in B(X,Y)$ such that
    $\norm{M_nx - Mx}_Y\to 0$ for all $x\in X$. 
\end{proposition}
\begin{proof}
    Set $Mx = \lim_{n\to\infty} M_nx$ for all $x\in X$. We check that $M\in B(X,Y)$. 
    Linearity is trivial; we check the boundedness. Let $f_n(x) = \norm{M_nx}_Y$. 
    Then $f_n$ is sub-additive and $f_n(\alpha x) = \abs{\alpha}f_n(x)$ for all $\alpha\in\R$. 
    If $x_k\to x$, 
    \begin{equation*}
        f_n(x_k) = \norm{M_nx_k}_Y\to\norm{Mx_k}_Y = f_n(x)
    \end{equation*}
    for any fixed $n$ as $k\to\infty$; $f_n$ is continuous. Now for any fixed $x\in X$, 
    $\sup_n f_n(x) = \sup_n \norm{M_nx}\leq C(x)$ by the strong convergence. It follows 
    from the uniform boundedness principle that there is $C_0<\infty$ such that 
    $\abs{f_n(x)}\leq C_0\norm{x}_X$ for all $n$. Thus 
    \begin{equation*}
        \norm{Mx}_Y = \lim_{n\to\infty} \norm{M_nx}_Y \leq C_0\norm{x}_X.
    \end{equation*}
    Hence $\norm{M}\leq C_0$ and $M\in B(X,Y)$.
\end{proof}

\begin{definition}
    A sequence $\set{M_n}\subset B(X,Y)$ \textbf{converges weakly} if for all 
    $x\in X$, $M_nx\wto y\in Y$ for some $y$. 
\end{definition}

\begin{proposition}
    If $\set{M_n}\subset B(X,Y)$ converges weakly, then there is an $M\in B(X,Y)$ such that 
    $M_nx\wto Mx$ for all $x\in X$.
\end{proposition}
\begin{proof}
    Set $Mx = \lim_{n\to\infty} M_nx$ for all $x\in X$. We check that $M\in B(X,Y)$. 
    Linearity is trivial; we check the boundedness. Without loss of genrality, we can 
    assume that $\norm{x}_X = 1$. Observe that $\set{M_nx}\subset Y$ 
    is a weakly convergence sequence and hence weakly sequentially compact; by 
    \cref{prop:w_seq_cpt_bd}, it is bounded. Thus there exists $C<\infty$ such that
    $\norm{M_nx}_Y\leq C = C\norm{x}$ for all $n$. Taking the limit, we have 
    $\norm{Mx}_Y = \lim_{n\to\infty} \norm{M_nx}_Y\leq C\norm{x}_X$. Hence $M\in B(X,Y)$.
    
    Lastly, we check the weak convergence. Indeed, for any $\ell\in Y'$, 
    $\ell(M_nx) = \ell(Mx)$ for all $x\in X$ since $M_nx\to Mx$ in $Y$. 
    Thus $M_nx\wto Mx$ in $Y$. 
\end{proof}